\documentclass{article}
\usepackage[utf8]{inputenc}
\usepackage{url}
\usepackage{amsmath}

\title{Math Reference}
\author{Oliver BÃ¶sing}
\date{May 2021}

\begin{document}

\maketitle

\section{Equations of Motion}

Let (X,Y,Z) be EME2000 fixed frame Cartesian co-ordinates. The orbit of an object is governed by the following equations of motion:

\begin{equation}
\begin{array}{ll}
     \ddot{X} = f_{Kep,X}(X,Y,Z)+f_{J2,X}(X,Y,Z)+f_{C22,X}(X,Y,Z,t)+f_{S22,X}(X,Y,Z,t)\\
    +f_{Moon,X}(X,Y,Z,t)+f_{Sun,X}(X,Y,Z,t)+f_{SRP,X}(X,Y,Z,t) \\
    \ddot{Y} = f_{Kep,Y}(X,Y,Z)+f_{J2,Y}(X,Y,Z)+f_{C22,Y}(X,Y,Z,t)+f_{S22,Y}(X,Y,Z,t)\\
    +f_{Moon,Y}(X,Y,Z,t)+f_{Sun,Y}(X,Y,Z,t)+f_{SRP,Y}(X,Y,Z,t) \\
    \ddot{Z} = f_{Kep,Z}(X,Y,Z)+f_{J2,Z}(X,Y,Z)+f_{C22,Z}(X,Y,Z,t)+f_{S22,Z}(X,Y,Z,t)\\
    +f_{Moon,Z}(X,Y,Z,t)+f_{Sun,Z}(X,Y,Z,t)+f_{SRP,Z}(X,Y,Z,t)
\end{array}
\end{equation}

\subsection{KepComponent}

\begin{equation}
\begin{array}{ll}
f_{Kep,X}(X,Y,Z) &= -{GM_E X\over (X^2+Y^2+Z^2)^{3/2}}\\
f_{Kep,Y}(X,Y,Z) &= -{GM_E Y\over (X^2+Y^2+Z^2)^{3/2}}\\
f_{Kep,Z}(X,Y,Z) &= -{GM_E Z\over (X^2+Y^2+Z^2)^{3/2}}
\end{array}
\end{equation}

\subsubsection{Implementation details}

First calculate shared factor

\begin{equation}
\begin{array}{ll}
d &= {1\over (X^2+Y^2+Z^2)^{3/2}}
\end{array}
\end{equation}

After that calculate

\begin{equation}
\begin{array}{ll}
f_{Kep,X}(X,Y,Z) &= -GM_EdX\\
f_{Kep,Y}(X,Y,Z) &= -GM_EdY\\
f_{Kep,Z}(X,Y,Z) &= -GM_EdZ
\end{array}
\end{equation}

\subsection{J2Component}

\begin{equation}
\begin{array}{ll}
f_{J2,X}(X,Y,Z) &=
{GM_ER_E^2\sqrt{5}C_{20} X\over 2(X^2+Y^2+Z^2)^{1/2}} \left({3\over(X^2+Y^2+Z^2)^2}-{15Z^2\over(X^2+Y^2+Z^2)^3}\right) \\
f_{J2,Y}(X,Y,Z) &=
{GM_ER_E^2\sqrt{5}C_{20} Y\over 2(X^2+Y^2+Z^2)^{1/2}} \left({3\over(X^2+Y^2+Z^2)^2}-{15Z^2\over(X^2+Y^2+Z^2)^3}\right) \\
f_{J2,Z}(X,Y,Z) &=
{GM_ER_E^2\sqrt{5}C_{20} Z\over 2(X^2+Y^2+Z^2)^{1/2}} \left({9\over(X^2+Y^2+Z^2)^2}-{15Z^2\over(X^2+Y^2+Z^2)^3}\right)
\end{array}
\end{equation}

\subsubsection{Implementation details}

Precalculate constant factor

\begin{equation}
\begin{array}{ll}
f &= {GM_ER_E^2\sqrt{5}C_{20}\over 2}
\end{array}
\end{equation}

Per (X,Y,Z) calculate

\begin{equation}
\begin{array}{ll}
d_1 &= {f{1\over \sqrt{X^2+Y^2+Z^2}}} \\
d_2 &= {1\over (X^2+Y^2+Z^2)^2} \\
s &= {15Z^2\over (X^2+Y^2+Z^2)^3}
\end{array}
\end{equation}

And

\begin{equation}
\begin{array}{ll}
f_{J2,X}(X,Y,Z) &= {d_1X\left({3d_2}-{s}\right)} \\
f_{J2,Y}(X,Y,Z) &= {d_1Y\left({3d_2}-{s}\right)} \\
f_{J2,Z}(X,Y,Z) &= {d_1Z\left({9d_2}-{s}\right)}
\end{array}
\end{equation}

\subsection{C22S22Component}

\begin{equation}
\begin{array}{ll}
f_{C22,X}(X,Y,Z,t) &= f_{C22,x}(x,y,z)\cos(\theta_G+\nu_Et) - f_{C22,y}(x,y,z)\sin(\theta_G+\nu_Et) \\
f_{C22,Y}(X,Y,Z,t) &= f_{C22,x}(x,y,z)\sin(\theta_G+\nu_Et) + f_{C22,y}(x,y,z)\cos(\theta_G+\nu_Et) \\
f_{C22,Z}(X,Y,Z,t) &= f_{C22,z}(x,y,z)\\
f_{S22,X}(X,Y,Z,t) &= f_{S22,x}(x,y,z)\cos(\theta_G+\nu_Et) - f_{S22,y}(x,y,z)\sin(\theta_G+\nu_Et) \\
f_{S22,Y}(X,Y,Z,t) &= f_{S22,x}(x,y,z)\sin(\theta_G+\nu_Et) + f_{S22,y}(x,y,z)\cos(\theta_G+\nu_Et) \\
f_{S22,Z}(X,Y,Z,t) &= f_{S22,z}(x,y,z)
\end{array}
\end{equation}

with

\begin{equation}
\begin{array}{ll}
x&=~X\cos(\theta_G+\nu_Et)+Y\sin(\theta_G+\nu_Et) \\
y&=-X\sin(\theta_G+\nu_Et)+Y\cos(\theta_G+\nu_Et) \\
z&=~Z
\end{array}
\end{equation}

and

\begin{equation}
\begin{array}{ll}
f_{C22,x}(x,y,z) &= {5GM_ER_E^2\sqrt{15}C_{22}x(y^2-x^2)\over 2(x^2+y^2+z^2)^{7/2}}+{GM_ER_E^2\sqrt{15}C_{22}x\over(x^2+y^2+z^2)^{5/2}} \\
f_{C22,y}(x,y,z) &= {5GM_ER_E^2\sqrt{15}C_{22}y(y^2-x^2)\over 2(x^2+y^2+z^2)^{7/2}}-{GM_ER_E^2\sqrt{15}C_{22}y\over(x^2+y^2+z^2)^{5/2}} \\
f_{C22,z}(x,y,z) &= {5GM_ER_E^2\sqrt{15}C_{22}z(y^2-x^2)\over 2(x^2+y^2+z^2)^{7/2}}\\
f_{S22,x}(x,y,z) &= -{5GM_ER_E^2\sqrt{15}S_{22}x^2y\over (x^2+y^2+z^2)^{7/2}}+{GM_ER_E^2\sqrt{15}S_{22}y\over(x^2+y^2+z^2)^{5/2}} \\
f_{S22,y}(x,y,z) &= -{5GM_ER_E^2\sqrt{15}S_{22}xy^2\over (x^2+y^2+z^2)^{7/2}}+{GM_ER_E^2\sqrt{15}S_{22}x\over(x^2+y^2+z^2)^{5/2}} \\
f_{S22,z}(x,y,z) &= -{5GM_ER_E^2\sqrt{15}S_{22}xyz\over (x^2+y^2+z^2)^{7/2}}
\end{array}
\end{equation}

\subsubsection{Implementation details}

Precalculate constant factors

\begin{equation}
\begin{array}{ll}
f &= {GM_ER_E^2\sqrt{15}}
\end{array}
\end{equation}

\begin{equation}
\begin{array}{ll}
f_{C_{22_2}} &= {GM_ER_E^2\sqrt{15}C_{22}} \\
             &= fC_{22} \\
f_{C_{22_1}} &= {{5GM_ER_E^2\sqrt{15}C_{22}} \over {2}} \\
             &= f_{C_{22_2}}\left( 5 \over 2\right)
\end{array}
\end{equation}

\begin{equation}
\begin{array}{ll}
f_{S_{22_2}} &= {GM_ER_E^2\sqrt{15}S_{22}} \\
             &= fS_{22} \\
f_{S_{22_1}} &= {-5GM_ER_E^2\sqrt{15}S_{22}} \\
             &= -5f_{S22_2}
\end{array}
\end{equation}

Per time step calculate

\begin{equation}
\begin{array}{ll}
f_{sin} &= \sin(\theta_G+\nu_Et) \\
f_{cos} &= \cos(\theta_G+\nu_Et)
\end{array}
\end{equation}

Per (X,Y,Z) calculate

\begin{equation}
\begin{array}{ll}
x&=~Xf_{cos}+Yf_{sin} \\
y&=-Xf_{sin}+Yf_{cos} \\
z&=~Z
\end{array}
\end{equation}

Shared terms

\begin{equation}
\begin{array}{ll}
n_{C_{22}} &= f_{C_{22_1}}(y^2-x^2) \\
n_{S_{22}} &= f_{S_{22_1}}xy
\end{array}
\end{equation}

\begin{equation}
\begin{array}{ll}
d_1 &= {1 \over \sqrt{(x^2+y^2+z^2)^7}} \\
d_2 &= {1 \over \sqrt{(x^2+y^2+z^2)^5}}
\end{array}
\end{equation}

Calculate

\begin{equation}
\begin{array}{ll}
f_{C22,x}(x,y,z) &= n_{C_{22}}xd_1 + f_{C_{22_2}}xd_2 \\
f_{C22,y}(x,y,z) &= n_{C_{22}}yd_1 + f_{C_{22_2}}yd_2 \\
f_{S22,x}(x,y,z) &= n_{S_{22}}xd_1 + f_{S_{22_2}}yd_2 \\
f_{S22,y}(x,y,z) &= n_{S_{22}}yd_1 + f_{S_{22_2}}xd_2
\end{array}
\end{equation}

\begin{equation}
\begin{array}{ll}
f_{C22,X}(X,Y,Z,t) &= f_{C22,x}(x,y,z)f_{cos} - f_{C22,y}(x,y,z)f_{sin} \\
f_{C22,Y}(X,Y,Z,t) &= f_{C22,x}(x,y,z)f_{sin} + f_{C22,y}(x,y,z)f_{cos} \\
f_{C22,Z}(X,Y,Z,t) &= n_{C_{22}}zd_1 \\
f_{S22,X}(X,Y,Z,t) &= f_{S22,x}(x,y,z)f_{cos} - f_{S22,y}(x,y,z)f_{sin} \\
f_{S22,Y}(X,Y,Z,t) &= f_{S22,x}(x,y,z)f_{sin} + f_{S22,y}(x,y,z)f_{cos} \\
f_{S22,Z}(X,Y,Z,t) &= n_{S_{22}}zd_1
\end{array}
\end{equation}

\subsection{SolComponent}

\begin{equation}
\begin{array}{ll}
f_{Sun,X}(X,Y,Z,t) &=-G M_\odot\left(
{(X-X_\odot)\over [(X-X_\odot)^2+(Y-Y_\odot)^2+(Z-Z_\odot)^2]^{3/2}}
+{X_\odot\over(X_\odot^2+Y_\odot^2+Z_\odot^2)^{3/2}} \right)\\
f_{Sun,Y}(X,Y,Z,t) &=-G M_\odot\left(
{(Y-Y_\odot)\over [(X-X_\odot)^2+(Y-Y_\odot)^2+(Z-Z_\odot)^2]^{3/2}}
+{Y_\odot\over(X_\odot^2+Y_\odot^2+Z_\odot^2)^{3/2}} \right)\\
f_{Sun,Z}(X,Y,Z,t) &=-G M_\odot\left(
{(Z-Z_\odot)\over [(X-X_\odot)^2+(Y-Y_\odot)^2+(Z-Z_\odot)^2]^{3/2}}
+{Z_\odot\over(X_\odot^2+Y_\odot^2+Z_\odot^2)^{3/2}} \right)
\end{array}
\end{equation}

where

\begin{equation}
\begin{pmatrix}
X_\odot\\
Y_\odot\\
Z_\odot
\end{pmatrix} = \begin{pmatrix}
r_\odot \cos \lambda_\odot\\
r_\odot \sin \lambda_\odot \cos \varepsilon\\
r_\odot \sin \lambda_\odot \sin \varepsilon
\end{pmatrix}
\end{equation}

with

\begin{equation}
\begin{array}{ll}
\lambda_\odot &= \Omega_\odot+\omega_\odot+\ell_{\odot}+\left(
{6892\over3600} \sin \ell_{\odot} + {72\over 3600} \sin 2\ell_{\odot}\right)\\
r_\odot[10^6\mbox{km}] &=149.619-2.499 \cos \ell_{\odot} - 0.021 \cos 2\ell_{\odot}\\
\ell_{\odot} &= \varphi_{\odot,0}+\nu_\odot t
\end{array}
\end{equation}

\subsubsection{Implementation details}

Per time step calculate

\begin{equation}
\begin{array}{ll}
\lambda_\odot &= \Omega_\odot+\omega_\odot+\ell_{\odot}+\left(
{6892\over3600} \sin \ell_{\odot} + {72\over 3600} \sin 2\ell_{\odot}\right)\\
r_\odot[10^6\mbox{km}] &=149.619-2.499 \cos \ell_{\odot} - 0.021 \cos 2\ell_{\odot}\\
\ell_{\odot} &= \varphi_{\odot,0}+\nu_\odot t
\end{array}
\end{equation}

\begin{equation}
\begin{array}{ll}
f_{X_{\odot}} &=\cos \lambda_\odot \\
f_{Y_{\odot}} &=\sin \lambda_\odot \cos \varepsilon \\
f_{Z_{\odot}} &=\sin \lambda_\odot \sin \varepsilon
\end{array}
\end{equation}

\begin{equation}
\begin{array}{ll}
X_{\odot} &= f_{X_{\odot}}r_\odot\times 10^{6} \\
Y_{\odot} &= f_{Y_{\odot}}r_\odot\times 10^{6} \\
Z_{\odot} &= f_{Z_{\odot}}r_\odot\times 10^{6} \\
\end{array}
\end{equation}

\begin{equation}
\begin{array}{ll}
d_1 &= {1 \over \sqrt{(X_\odot^2+Y_\odot^2+Z_\odot^2)^3}}
\end{array}
\end{equation}

\begin{equation}
\begin{array}{ll}
P_{X_{\odot}} &= d_1X_{\odot} \\
P_{Y_{\odot}} &= d_1Y_{\odot} \\
P_{Z_{\odot}} &= d_1Z_{\odot}
\end{array}
\end{equation}

Per (X,Y,Z) calculate

\begin{equation}
\begin{array}{ll}
d_2 &= {1 \over \sqrt{((X-X_\odot)^2+(Y-Y_\odot)^2+(Z-Z_\odot)^2)^3}}
\end{array}
\end{equation}

\begin{equation}
\begin{array}{ll}
f_{Sun,X}(X,Y,Z,t) &=-GM_\odot(d_2(X-X_{\odot})+P_{X_{\odot}}) \\
f_{Sun,Y}(X,Y,Z,t) &=-GM_\odot(d_2(Y-Y_{\odot})+P_{Y_{\odot}}) \\
f_{Sun,Z}(X,Y,Z,t) &=-GM_\odot(d_2(Z-Z_{\odot})+P_{Z_{\odot}})
\end{array}
\end{equation}

\subsection{LunComponent}

\begin{equation}
\begin{array}{ll}
f_{Moon,X}(X,Y,Z,t) &=-G M_{\mathcal M}\left({(X-X_{\mathcal M})\over [(X-X_{\mathcal M})^2+(Y-Y_{\mathcal M})^2+(Z-Z_{\mathcal M})^2]^{3/2}}
+{X_{\mathcal M}\over(X_{\mathcal M}^2+Y_{\mathcal M}^2+Z_{\mathcal M}^2)^{3/2}} \right)\\
f_{Moon,Y}(X,Y,Z,t) &=-G M_{\mathcal M}\left({(Y-Y_{\mathcal M})\over [(X-X_{\mathcal M})^2+(Y-Y_{\mathcal M})^2+(Z-Z_{\mathcal M})^2]^{3/2}}
+{Y_{\mathcal M}\over(X_{\mathcal M}^2+Y_{\mathcal M}^2+Z_{\mathcal M}^2)^{3/2}} \right)\\
f_{Moon,Z}(X,Y,Z,t) &=-G M_{\mathcal M}\left({(Z-Z_{\mathcal M})\over [(X-X_{\mathcal M})^2+(Y-Y_{\mathcal M})^2+(Z-Z_{\mathcal M})^2]^{3/2}}
+{Z_{\mathcal M}\over(X_{\mathcal M}^2+Y_{\mathcal M}^2+Z_{\mathcal M}^2)^{3/2}} \right)
\end{array}
\end{equation}

where

\begin{equation}
\begin{pmatrix}
X_{\mathcal M}\\
Y_{\mathcal M}\\
Z_{\mathcal M}
\end{pmatrix} = \begin{pmatrix}
1 & 0 & 0 \\
0 & \cos\varepsilon & -\sin\varepsilon\\
0 & \sin\varepsilon & \cos\varepsilon
\end{pmatrix} \cdot \begin{pmatrix}
r_{{\mathcal M}} \cos \lambda_{{\mathcal M}} \cos \beta_{{\mathcal M}}\\
r_{{\mathcal M}} \sin \lambda_{{\mathcal M}} \cos \beta_{{\mathcal M}}\\
r_{{\mathcal M}} \sin \beta_{{\mathcal M}}
\end{pmatrix}
\end{equation}

with

\begin{equation}
\begin{array}{ll}
r_{{\mathcal M}}[\mbox{km}] &= 385000-20905 \cos(l_{{{\mathcal M}}})-3699 \cos(2 D_{{{\mathcal M}}}-l_{{{\mathcal M}}}) \\
&-2956 \cos(2 D_{{{\mathcal M}}})-570 \cos(2 l_{{{\mathcal M}}})\\
&+246\cos(2 l_{{{\mathcal M}}}-2 D_{{{\mathcal M}}})-205 \cos(l'_{{{\mathcal M}}}-2 D_{{{\mathcal M}}})\\
&-171 \cos(l_{{{\mathcal M}}}+2 D_{{{\mathcal M}}})\\
&-152 \cos(l_{{{\mathcal M}}}+l'_{{{\mathcal M}}}-2 D_{{{\mathcal M}}})
\end{array}
\end{equation}
\begin{equation}
\begin{array}{ll}
\begin{array}{ll}
\lambda_{\mathcal M} &= L_0+ ( {22640\over 3600} \sin(l_{\mathcal M})
+ {769\over 3600} \sin(2 l_{\mathcal M})\\
&- {4856\over 3600} \sin(l_{\mathcal M} - 2 D_{\mathcal M})
+ {2370\over 3600} \sin(2 D_{\mathcal M})\\
&- {668\over 3600} \sin(l'_{\mathcal M}) - {412\over 3600} \sin(2 F_{\mathcal M})\\
&- {212\over 3600} \sin(2 l_{\mathcal M} - 2 D_{\mathcal M})
- {206\over 3600} \sin(l_{\mathcal M} + l'_{\mathcal M} - 2 D_{\mathcal M})\\
&+ {192\over 3600} \sin(l_{\mathcal M} + 2 D_{\mathcal M})
- {165\over 3600} \sin(l'_{\mathcal M} - 2 D_{\mathcal M})\\
&+ {148\over 3600} \sin(l_{\mathcal M} - l'_{\mathcal M})
- {125\over 3600} \sin(D_{\mathcal M})\\
&- {110\over 3600} \sin(l_{\mathcal M} + l'_{\mathcal M})
- {55\over 3600} \sin(2 F_{\mathcal M} - 2 D_{\mathcal M}) )
\end{array}
\end{array}
\end{equation}
\begin{equation}
\begin{array}{ll}
\beta_{{\mathcal M}} &= ( {18520\over 3600} \sin\left(F_{{\mathcal M}}
+ \lambda_{{\mathcal M}}-L_0 +  ( {412\over 3600} \sin(2F_{{\mathcal M}})
+ {541\over 3600} \sin(l'_{{\mathcal M}})) \right)\\
&- {526\over 3600} \sin(F_{{\mathcal M}} - 2D_{{\mathcal M}})\\
&+ {44\over 3600} \sin(l_{{\mathcal M}} + F_{{\mathcal M}} - 2D_{{\mathcal M}})
- {31\over 3600} \sin(-l_{{\mathcal M}} + F_{{\mathcal M}} - 2D_{{\mathcal M}})\\
&- {25\over 3600} \sin(-2l_{{\mathcal M}} + F_{\mathcal M})
- {23\over 3600} \sin(l'_{\mathcal M}
+ F_{\mathcal M} - 2D_{\mathcal M})\\
&+ {21\over 3600} \sin(-l_{\mathcal M} + F_{\mathcal M})
+ {11\over 3600} \sin(-l'_{\mathcal M} + F_{\mathcal M} - 2D_{\mathcal M}) )
\end{array}
\end{equation}

and

\begin{equation}
\begin{array}{ll}
\varphi_{M}&=\nu_\odot t\\
\varphi_{M_a}&=\nu_{M_a}t\\
\varphi_{M_p}&=\nu_{M_p}t\\
\varphi_{M_S}&=\nu_{M_s}t\\
L_0&=\varphi_{M_p}+\varphi_{M_a}+ (218.31617)\\
l_{\mathcal M}&=\varphi_{M_a}+ (134.96292)\\
l'_{\mathcal M}&=\ell_{\odot}=\varphi_M+ (357.52543)\\
F_{\mathcal M}&=\varphi_{M_p}+\varphi_{M_a}+\varphi_{M_S}+ (93.27283)\\
D_{\mathcal M}&=\varphi_{M_p}+\varphi_{M_a}-\varphi_{M}+ (297.85027)
\end{array}
\end{equation}

\subsubsection{Implementation details}

Per time step calculate

\begin{equation}
\begin{array}{ll}
\varphi_{M}&=\nu_\odot t\\
\varphi_{M_a}&=\nu_{M_a}t\\
\varphi_{M_p}&=\nu_{M_p}t\\
\varphi_{M_S}&=\nu_{M_s}t\\
L_0&=\varphi_{M_p}+\varphi_{M_a}+(218.31617)\\
l_{\mathcal M}&=\varphi_{M_a}+(134.96292)\\
l'_{\mathcal M}&=\ell_{\odot}=\varphi_M+ (357.52543)\\
F_{\mathcal M}&=\varphi_{M_p}+\varphi_{M_a}+\varphi_{M_S}+ (93.27283)\\
D_{\mathcal M}&=\varphi_{M_p}+\varphi_{M_a}-\varphi_{M}+  (297.85027)
\end{array}
\end{equation}

Rearrangement of terms clarifies order of executed calculations

\begin{equation}
\begin{array}{ll}
r_{{\mathcal M}} &= -152 \cos(l_{{{\mathcal M}}}+l'_{{{\mathcal M}}}-2 D_{{{\mathcal M}}})\\
&-171 \cos(l_{{{\mathcal M}}}+2 D_{{{\mathcal M}}})\\
&-205 \cos(l'_{{{\mathcal M}}}-2 D_{{{\mathcal M}}})\\
&+246 \cos(2 l_{{{\mathcal M}}}-2 D_{{{\mathcal M}}})\\
&-2956 \cos(2 D_{{{\mathcal M}}})\\
&-3699 \cos(2 D_{{{\mathcal M}}}-l_{{{\mathcal M}}}) \\
&-20905 \cos(l_{{{\mathcal M}}})\\
&+ 385000
\end{array}
\end{equation}
\begin{equation}
\begin{array}{ll}
\lambda_{\mathcal M} &= -{55\over 3600} \sin(2 F_{\mathcal M} - 2 D_{\mathcal M}) \\
&- {110\over 3600} \sin(l_{\mathcal M} + l'_{\mathcal M})\\
&- {125\over 3600} \sin(D_{\mathcal M})\\
&+ {148\over 3600} \sin(l_{\mathcal M} - l'_{\mathcal M})\\
&- {165\over 3600} \sin(l'_{\mathcal M} - 2 D_{\mathcal M})\\
&+ {192\over 3600} \sin(l_{\mathcal M} + 2 D_{\mathcal M})\\
&- {206\over 3600} \sin(l_{\mathcal M} + l'_{\mathcal M} - 2 D_{\mathcal M})\\
&- {212\over 3600} \sin(2 l_{\mathcal M} - 2 D_{\mathcal M}) \\
&- {412\over 3600} \sin(2 F_{\mathcal M})\\
&- {668\over 3600} \sin(l'_{\mathcal M}) \\
&+ {769\over 3600} \sin(2 l_{\mathcal M})\\
&+ {2370\over 3600} \sin(2 D_{\mathcal M})\\
&- {4856\over 3600} \sin(l_{\mathcal M} - 2 D_{\mathcal M}) \\
&+ {22640\over 3600} \sin(l_{\mathcal M})\\
&+ L_0
\end{array}
\end{equation}
\begin{equation}
\begin{array}{ll}
\beta_{{\mathcal M}} &= {11\over 3600} \sin(-l'_{\mathcal M} + F_{\mathcal M} - 2D_{\mathcal M})\\
&+ {21\over 3600} \sin(-l_{\mathcal M} + F_{\mathcal M})+ F_{\mathcal M} - 2D_{\mathcal M})\\
&- {23\over 3600} \sin(l'_{\mathcal M} \\
&- {25\over 3600} \sin(-2l_{{\mathcal M}} + F_{\mathcal M})\\
&- {31\over 3600} \sin(-l_{{\mathcal M}} + F_{{\mathcal M}} - 2D_{{\mathcal M}})\\
&+ {44\over 3600} \sin(l_{{\mathcal M}} + F_{{\mathcal M}} - 2D_{{\mathcal M}}) \\
&- {526\over 3600} \sin(F_{{\mathcal M}} - 2D_{{\mathcal M}})\\
&+ {18520\over 3600} \sin\left(F_{{\mathcal M}} + \lambda_{{\mathcal M}}-L_0 + ( {412\over 3600} \sin(2F_{{\mathcal M}} + {541\over 3600} \sin(l'_{{\mathcal M}})) \right)\\
\end{array}
\end{equation}

\begin{equation}
\begin{array}{ll}
f_{\mathcal M,1} &= \cos{\lambda_{\mathcal M}}\cos{\beta_{\mathcal M}} \\
f_{\mathcal M,2} &= \sin{\lambda_{\mathcal M}}\cos{\beta_{\mathcal M}} \\
f_{\mathcal M,3} &= \sin{\beta_{\mathcal M}}
\end{array}
\end{equation}

\begin{equation}
\begin{array}{ll}
X_{\mathcal M} &= f_{\mathcal M,1}r_{\mathcal M} \\
Y_{\mathcal M} &= (f_{\mathcal M,2}\cos\varepsilon - f_{\mathcal M,3}\sin\varepsilon)r_{\mathcal M} \\
Z_{\mathcal M} &= (f_{\mathcal M,2}\sin\varepsilon + f_{\mathcal M,3}\cos\varepsilon)r_{\mathcal M}
\end{array}
\end{equation}

\begin{equation}
\begin{array}{ll}
d_1 &= {1 \over \sqrt{(X_\mathcal M^2+Y_\mathcal M^2+Z_\mathcal M^2)^3}}
\end{array}
\end{equation}

\begin{equation}
\begin{array}{ll}
P_{X_{\mathcal M}} &= d_1X_{\mathcal M} \\
P_{Y_{\mathcal M}} &= d_1Y_{\mathcal M} \\
P_{Z_{\mathcal M}} &= d_1Z_{\mathcal M}
\end{array}
\end{equation}

Per (X,Y,Z) calculate

\begin{equation}
\begin{array}{ll}
d_2 &= {1 \over \sqrt{((X-X_\mathcal M)^2+(Y-Y_\mathcal M)^2+(Z-Z_\mathcal M)^2)^3}}
\end{array}
\end{equation}

\begin{equation}
\begin{array}{ll}
f_{Moon,X}(X,Y,Z,t) &=-GM_\mathcal M(d_2(X-X_{\mathcal M})+P_{X_{\mathcal M}}) \\
f_{Moon,Y}(X,Y,Z,t) &=-GM_\mathcal M(d_2(Y-Y_{\mathcal M})+P_{Y_{\mathcal M}}) \\
f_{Moon,Z}(X,Y,Z,t) &=-GM_\mathcal M(d_2(Z-Z_{\mathcal M})+P_{Z_{\mathcal M}})
\end{array}
\end{equation}

\subsection{SRPComponent}

\begin{equation}
\begin{array}{ll}
f_{SRP,X}(X,Y,Z,t) &= AOM
{P_{SRP}a_\odot^2(X-X_\odot)\over [(X-X_\odot)^2+(Y-Y_\odot)^2+(Z-Z_\odot)^2]^{3/2}}\\
f_{SRP,Y}(X,Y,Z,t) &= AOM
{P_{SRP}a_\odot^2(Y-Y_\odot)\over [(X-X_\odot)^2+(Y-Y_\odot)^2+(Z-Z_\odot)^2]^{3/2}}\\
f_{SRP,Z}(X,Y,Z,t) &= AOM
{P_{SRP}a_\odot^2(Z-Z_\odot)\over [(X-X_\odot)^2+(Y-Y_\odot)^2+(Z-Z_\odot)^2]^{3/2}}
\end{array}
\end{equation}

\subsubsection{Implementation details}

Precalculated constant factor

\begin{equation}
\begin{array}{ll}
f &= P_{SRP}a_\odot^2
\end{array}
\end{equation}

Per time step

Use \(X_{\odot}\), \(Y_{\odot}\) and \(Z_{\odot}\) from SolComponent

Per (X,Y,Z) calculate

\begin{equation}
\begin{array}{ll}
d &= {1 \over \sqrt{((X-X_\odot)^2+(Y-Y_\odot)^2+(Z-Z_\odot)^2)^3}}
\end{array}
\end{equation}

\begin{equation}
\begin{array}{ll}
f_{SRP,X}(X,Y,Z,t) &=AOM(df(X-X_{\odot})) \\
f_{SRP,Y}(X,Y,Z,t) &=AOM(df(Y-Y_{\odot})) \\
f_{SRP,Z}(X,Y,Z,t) &=AOM(df(Z-Z_{\odot}))
\end{array}
\end{equation}

\subsection{DragComponent}

\subsubsection{Implementation details}

\section{Constants}

\begin{align}
%\begin{array}{ll}
GM_E &=3.986004407799724\times 10^5 km^3 sec^{-2} \\
GM_\odot &= 1.32712440018\times 10^{11}km^3 sec^{-2} \\
GM_{\mathcal M} &=4.9028\times 10^{3}km^3 sec^{-2} \\
R_E &=6378.1363 km\\
C_{20} &= -4.84165371736\times 10^{-4}\\
C_{22} &= 2.43914352398\times 10^{-6}\\
S_{22} &=-1.40016683654\times 10^{-6}\\
\theta_G &= (280.4606)\\
\nu_E  &=(4.178074622024230\times 10^{-3})\\
\nu_\odot &=  (1.1407410259335311\times 10^{-5})\\
\nu_{M_a} &=  (1.512151961904581\times 10^{-4})\\
\nu_{M_p} &=  (1.2893925235125941\times 10^{-6})\\
\nu_{M_s} &=  (6.128913003523574\times 10^{-7})\\
a_\odot &= 1.49619 \times 10^8 km\\
\varepsilon&= (23.4392911)\\
\varphi_{\odot,0} &= (357.5256)\\
\Omega_\odot + \omega_\odot &=  (282.94) \\
P_{SRP} &=4.56\times 10^{-6}
%\end{array}
\end{align}

\end{document}
